theories/syntax.v
@@ -6,32 +6,32 @@ Require Import Coq.ZArith.ZArith.
 Require Import tactics.
 
 Inductive op :=
-    | Add
-    | Eq
+  | Add
+  | Eq
 .
 
 Inductive term :=
-    | Var (x: var)
-    | FreeVar (x: string) (* external variables *)
-    | App (t1 t2: term)
-    | Lam (t: {bind term})
-    | Default (ts: list term) (tj tc: term)
-    | Empty
-    | Conflict
+  | Var (x: var)
+  | FreeVar (x: string) (* external variables *)
+  | App (t1 t2: term)
+  | Lam (t: {bind term})
+  | Default (ts: list term) (tj tc: term)
+  | Empty
+  | Conflict
 
-    | Value (v: value)
-    | Binop (op: op) (t1 t2: term)
+  | Value (v: value)
+  | Binop (op: op) (t1 t2: term)
 
-    | Match_ (u t1: term) (t2: {bind term})
-    | ENone
-    | ESome (t: term)
+  | Match_ (u t1: term) (t2: {bind term})
+  | ENone
+  | ESome (t: term)
 
 with value :=
-    | Bool (b: bool)
-    | Int (i: Z)
-    | Closure (t: {bind term}) (sigma: list value)
-    | VNone
-    | VSome (v: value)
+  | Bool (b: bool)
+  | Int (i: Z)
+  | Closure (t: {bind term}) (sigma: list value)
+  | VNone
+  | VSome (v: value)
 .
 
 #[export] Instance Ids_term : Ids term. derive. Defined.
@@ -40,7 +40,7 @@ with value :=
 #[export] Instance SubstLemmas_term : SubstLemmas term. derive. Qed.
 
 Lemma ids_inj:
-    forall x y, ids x = ids y -> x = y.
+  forall x y, ids x = ids y -> x = y.
 intros; inj; eauto.
 Qed.
 
@@ -48,16 +48,146 @@ Qed.
 
 
 Definition get_op op i1 i2:=
-    match op, i1, i2 with
-    | Add, Int i1, Int i2 => Some (Int (Z.add i1 i2))
-    | Eq, Int i1, Int i2 => Some (Bool (Z.eqb i1 i2))
-    | _, _, _ => None
-    end
-.
+  match op, i1, i2 with
+  | Add, Int i1, Int i2 => Some (Int (Z.add i1 i2))
+  | Eq, Int i1, Int i2 => Some (Bool (Z.eqb i1 i2))
+  | _, _, _ => None
+  end.
 
 Definition value_eqb (v1 v2 : value) : bool :=
-    match v1, v2 with
-    | Bool b1, Bool b2 => Bool.eqb b1 b2
-    | Int i1, Int i2 => Z.eqb i1 i2
-    | _, _ => false
-    end.
+  match v1, v2 with
+  | Bool b1, Bool b2 => Bool.eqb b1 b2
+  | Int i1, Int i2 => Z.eqb i1 i2
+  | _, _ => false
+  end.
+
+Require Import Autosubst_FreeVars.
+
+Lemma lift_inj_EVar:
+  forall t x,
+  lift 1 t = Var (S x) <-> t = Var x.
+Proof.
+  split; intros.
+  { eauto using lift_inj. }
+  { subst. eauto. }
+Qed.
+
+Lemma fv_Var_eq:
+  forall k x,
+  fv k (Var x) <-> x < k.
+Proof.
+  unfold fv. asimpl. induction k; intros.
+  (* Base case. *)
+  { asimpl. split; intros; exfalso.
+    { unfold ids, Ids_term in *. injections.
+      (* In Coq 8.12, this goal is solved by [lia], but not in Coq 8.10. *)
+      eapply Nat.neq_succ_diag_l. eauto. }
+    { lia. }
+  }
+  (* Step. *)
+  { destruct x; asimpl.
+    { split; intros. { lia. } { reflexivity. } }
+    rewrite lift_inj_EVar. rewrite IHk. lia. }
+Qed.
+
+Lemma fv_Lam_eq:
+  forall k t,
+  fv k (Lam t) <-> fv (S k) t.
+Proof.
+  unfold fv. intros. asimpl. split; intros.
+  { injections. eauto. }
+  { unpack. congruence. }
+Qed.
+
+Lemma fv_App_eq:
+  forall k t1 t2,
+  fv k (App t1 t2) <-> fv k t1 /\ fv k t2.
+Proof.
+  unfold fv. intros. asimpl. split; intros.
+  { injections. eauto. }
+  { unpack. congruence. }
+Qed.
+
+Lemma fv_Binop_eq:
+  forall k op t1 t2,
+  fv k (Binop op t1 t2) <-> fv k t1 /\ fv k t2.
+Proof.
+  unfold fv. intros. asimpl. split; intros.
+  { injections. eauto. }
+  { unpack. congruence. }
+Qed.
+
+Lemma fv_Match_eq:
+  forall k tc t1 t2,
+  fv k (Match_ tc t1 t2) <-> fv k tc /\ fv k t1 /\ fv (S k) t2.
+Proof.
+  unfold fv. intros. asimpl. split; intros.
+  { injections. eauto. }
+  { unpack. congruence. }
+Qed.
+
+Lemma fv_VariantNone_eq:
+  forall k,
+  fv k ENone.
+Proof.
+  unfold fv. intros. now asimpl.
+Qed.
+
+Lemma fv_VariantSome_eq:
+  forall k t,
+  fv k (ESome t) <-> fv k t.
+Proof.
+  unfold fv. intros. asimpl. split; intros.
+  { injections. eauto. }
+  { congruence. }
+Qed.
+
+Lemma thing: forall ts sigma,
+  ts..[sigma] = ts <-> List.Forall (fun ti : term => ti.[sigma] = ti) ts.
+Proof.
+  induction ts.
+  * split; intros; eauto.
+  * split; intros; msimpl in *.
+    - injections.
+      econstructor; eauto.
+      { apply IHts. eauto. }
+    - inversion H.
+      f_equal; [eauto | now eapply IHts].
+Qed.
+
+Lemma fv_Default_eq:
+  forall k ts tj tc,
+  fv k (Default ts tj tc) <->
+    (List.Forall (fun ti => fv k ti) ts) /\ fv k tj /\ fv k tc.
+Proof.
+  unfold fv. intros. asimpl. split; intros.
+  { injections. repeat split; eauto.
+    { apply thing; assumption. }
+  }
+  { unpack. rewrite H0; rewrite H1.
+    remember (thing ts (upn k (ren (+1)))).
+    destruct i.
+    remember (e H).
+    rewrite e0.
+    reflexivity. }
+Qed.
+
+Lemma fv_Value_eq:
+  forall k v,
+  fv k (Value v) <-> True.
+Proof.
+  unfold fv. intros. asimpl. split; eauto.
+Qed.
+
+#[export]
+Hint Rewrite
+  fv_Var_eq
+  fv_Lam_eq
+  fv_App_eq
+  fv_VariantSome_eq
+  fv_VariantNone_eq
+  fv_Match_eq
+  fv_Binop_eq
+  fv_Default_eq
+  fv_Value_eq
+  : fv.
